---
title: "DSSF: N=1"
date: 2024-07-09
tags: ["Dynamical Spin Structure Factor"]
---

***Tags:*** {%for tag in page.tags %} *{{tag}}*{% if forloop.last != true %},{% endif %}{% endfor %}

# Example: One up-spin

We compute the **dynamical spin structure factor**. 
See [this post](/URSA23/2024/07/02/diss.html) for an intro and the derivation of the formulas in the general $$N$$ up-spin case.
The **dynamical spin structure factor** is given by the following formula

$$
S^{zz}(q, \omega) = \frac{1}{L} \sum_{j, j' =1}^L e^{- i q (j-j')} \int_{- \infty}^{\infty}dt e^{i \omega t} \langle S_j^z(t) S_{j'}^z(0) \rangle
$$

We focus on computing the observable inside the integrand. 
In [this post](/URSA23/2024/07/02/diss.html), we gave a formula for the observable:

$$
\begin{align}
& \langle S_j^z(t) S_{j'}^z \rangle = \langle \Psi \mid e^{i t H /\hbar } S_j^z e^{-i t H /\hbar } S_{j'}^z \mid \Psi \rangle\\
&= \frac{(-1)^{j' \notin y}}{2}  \sum_{x \in X} \frac{(-1)^{j \notin x}}{2} \sum_{[\zeta], [\xi] \in \Xi} \overline{\ell(y, \zeta) u(\zeta, x) } \ell(y, \xi) u(\xi, x) e^{-i t (E(\xi)- E(\zeta) )}.
\end{align}
$$

for the general $$N$$ up-spin case. 
We treat the $$N=1$$ case here, where many of the formulas simplify. 

## Functions

The **Bethe Equations** become

$$
\xi^L = 1.
$$

Thus, the solutions of the Bethe equations are the $$L^{th}$$ roots of unity.
We set $$ \eta = \exp(2 \pi i /L)$$ be a primitive $$L^{th}$$ roots of unity so that

$$
\eta^{k} = e^{2 \pi i k /L},
$$

for $$k=1, 2, \dots, L$$, are all the solutions of the Bethe equations.
Additionally, we have

$$
\begin{align}
u(\xi, x) = \xi^x, \quad \ell(y, \xi) = \xi^{-y}/L, \quad E(\xi) = \xi + \xi^{-1} - 2 \Delta
\end{align}
$$

## Computation

We have

$$
\begin{align}
& \langle S_j^z(t) S_{j'}^z \rangle = \langle \Psi \mid e^{i t H /\hbar } S_j^z e^{-i t H /\hbar } S_{j'}^z \mid \Psi \rangle\\
&= \frac{(-1)^{j' \notin y}}{2}  \sum_{x \in X} \frac{(-1)^{j \notin x}}{2} \sum_{[\zeta], [\xi] \in \Xi} \overline{\ell(y, \zeta) u(\zeta, x) } \ell(y, \xi) u(\xi, x) e^{-i t (E(\xi)- E(\zeta) )}\\
&= \frac{(-1)^{j' \neq y}}{2 }  \sum_{x = 1}^L \frac{(-1)^{j \neq x}}{2 } \sum_{k1, k2 = 1}^L L^{-2}\eta^{(k1-k2)(x-y)} e^{\tfrac{- i t}{\hbar}(\cos (2\pi k1/L) - \cos(2 \pi k2/L))}.
\end{align}
$$

Next, we integrate over time 

$$
\begin{align}
&\int_{- \infty}^{\infty}dt e^{i \omega t} \langle S_j^z(t) S_{j'}^z(0) \rangle\\
&= \lim_{T \rightarrow \infty} \int_{- T}^{T}dt e^{i \omega t} \langle S_j^z(t) S_{j'}^z(0) \rangle\\
&= \lim_{T \rightarrow \infty} \int_{- T}^{T}dt  \frac{(-1)^{j' \neq y}}{2 }  \sum_{x = 1}^L \frac{(-1)^{j \neq x}}{2 } \sum_{k1, k2 = 1}^L L^{-2}\eta^{(k1-k2)(x-y)} e^{\tfrac{- i t}{\hbar}(\cos (2\pi k1/L) - \cos(2 \pi k2/L) - \omega \hbar)}\\
&= \lim_{T \rightarrow \infty} \frac{(-1)^{j' \neq y}}{2 }  \sum_{x = 1}^L \frac{(-1)^{j \neq x}}{2 } \sum_{k1, k2 = 1}^L L^{-2}\eta^{(k1-k2)(x-y)} \int_{- T}^{T}dt e^{\tfrac{- i t}{\hbar}(\cos (2\pi k1/L) - \cos(2 \pi k2/L) - \omega \hbar)}\\
&= \lim_{T \rightarrow \infty} \frac{(-1)^{j' \neq y}}{2 }  \sum_{x = 1}^L \frac{(-1)^{j \neq x}}{2 } \sum_{k1, k2 = 1}^L \frac{- 2 \hbar L^{-2}\eta^{(k1-k2)(x-y)}}{\cos (2\pi k1/L) - \cos(2 \pi k2/L) - \omega \hbar}  \mathrm{Im} \left( e^{\tfrac{- i T}{\hbar}(\cos (2\pi k1/L) - \cos(2 \pi k2/L) - \omega \hbar)} \right) \\
&= \lim_{T \rightarrow \infty} \frac{(-1)^{j' \neq y}}{2 }  \sum_{x = 1}^L \frac{(-1)^{j \neq x}}{2 } \sum_{k1, k2 = 1}^L \frac{ 2 \hbar L^{-2}\eta^{(k1-k2)(x-y)} }{\cos (2\pi k1/L) - \cos(2 \pi k2/L) - \omega \hbar}  \sin \left( \tfrac{T}{\hbar}(\cos (2\pi k1/L) - \cos(2 \pi k2/L) - \omega \hbar) \right).
\end{align}
$$

At this point, it is hard to tell what the $$T \rightarrow \infty$$ will give. 

### Next Step

- Numerics using Mathematica



{% include utterances.html %}
